examples/nsl_pk/DY.Example.NSL.Protocol.Total.Proof.fst
@@ -21,30 +21,32 @@ val crypto_predicates_nsl: crypto_predicates crypto_usages_nsl
 let crypto_predicates_nsl = {
   default_crypto_predicates crypto_usages_nsl with
 
-  pkenc_pred = (fun tr pk msg ->
-    get_sk_usage pk == PkdecKey "NSL.PublicKey" /\
-    (exists prin. get_sk_label pk = principal_label prin /\ (
-      match parse message msg with
-      | Some (Msg1 msg1) -> (
-        let (alice, bob) = (msg1.alice, prin) in
-        event_triggered tr alice (Initiate1 alice bob msg1.n_a) /\
-        get_label msg1.n_a == join (principal_label alice) (principal_label bob)
-      )
-      | Some (Msg2 msg2) -> (
-        let (alice, bob) = (prin, msg2.bob) in
-        event_triggered tr bob (Respond1 alice bob msg2.n_a msg2.n_b) /\
-        get_label msg2.n_b == join (principal_label alice) (principal_label bob)
-      )
-      | Some (Msg3 msg3) -> (
-        let bob = prin in
-        exists alice n_a.
-          get_label msg3.n_b `can_flow tr` (principal_label alice) /\
-          event_triggered tr alice (Initiate2 alice bob n_a msg3.n_b)
-      )
-      | None -> False
-    ))
-  );
-  pkenc_pred_later = (fun tr1 tr2 pk msg -> ());
+  pkenc_pred = {
+    pred = (fun tr pk msg ->
+      get_sk_usage pk == PkdecKey "NSL.PublicKey" empty /\
+      (exists prin. get_sk_label pk = principal_label prin /\ (
+        match parse message msg with
+        | Some (Msg1 msg1) -> (
+          let (alice, bob) = (msg1.alice, prin) in
+          event_triggered tr alice (Initiate1 alice bob msg1.n_a) /\
+          get_label msg1.n_a == join (principal_label alice) (principal_label bob)
+        )
+        | Some (Msg2 msg2) -> (
+          let (alice, bob) = (prin, msg2.bob) in
+          event_triggered tr bob (Respond1 alice bob msg2.n_a msg2.n_b) /\
+          get_label msg2.n_b == join (principal_label alice) (principal_label bob)
+        )
+        | Some (Msg3 msg3) -> (
+          let bob = prin in
+          exists alice n_a.
+            get_label msg3.n_b `can_flow tr` (principal_label alice) /\
+            event_triggered tr alice (Initiate2 alice bob n_a msg3.n_b)
+        )
+        | None -> False
+      ))
+    );
+    pred_later = (fun tr1 tr2 pk msg -> ());
+  };
 }
 #pop-options
 
@@ -69,7 +71,7 @@ val compute_message1_proof:
     // From random generation
     PkNonce? (get_usage nonce) /\
     // From PKI invariants
-    is_encryption_key "NSL.PublicKey" (principal_label bob) tr pk_b
+    is_encryption_key (PkdecKey "NSL.PublicKey" empty) (principal_label bob) tr pk_b
   )
   (ensures is_publishable tr (compute_message1 alice bob pk_b n_a nonce))
 let compute_message1_proof tr alice bob pk_b n_a nonce =
@@ -89,7 +91,7 @@ val decode_message1_proof:
   Lemma
   (requires
     // From PrivateKeys invariants
-    is_decryption_key "NSL.PublicKey" (principal_label bob) tr sk_b /\
+    is_decryption_key (PkdecKey "NSL.PublicKey" empty) (principal_label bob) tr sk_b /\
     // From the network
     bytes_invariant tr msg_cipher
   )
@@ -125,7 +127,7 @@ val compute_message2_proof:
     // From the random generation
     PkNonce? (get_usage nonce) /\
     // From the PKI
-    is_encryption_key "NSL.PublicKey" (principal_label msg1.alice) tr pk_a
+    is_encryption_key (PkdecKey "NSL.PublicKey" empty) (principal_label msg1.alice) tr pk_a
   )
   (ensures
     is_publishable tr (compute_message2 bob msg1 pk_a n_b nonce)
@@ -149,7 +151,7 @@ val decode_message2_proof:
     // From the NSL state invariant
     is_secret (join (principal_label alice) (principal_label bob)) tr n_a /\
     // From the PrivateKeys invariant
-    is_decryption_key "NSL.PublicKey" (principal_label alice) tr sk_a /\
+    is_decryption_key (PkdecKey "NSL.PublicKey" empty) (principal_label alice) tr sk_a /\
     // From the network
     bytes_invariant tr msg_cipher
   )
@@ -188,7 +190,7 @@ val compute_message3_proof:
     // From the random generation
     PkNonce? (get_usage nonce) /\
     // From the PKI
-    is_encryption_key "NSL.PublicKey" (principal_label bob) tr pk_b
+    is_encryption_key (PkdecKey "NSL.PublicKey" empty) (principal_label bob) tr pk_b
   )
   (ensures
     is_publishable tr (compute_message3 alice bob pk_b n_b nonce)
@@ -213,7 +215,7 @@ val decode_message3_proof:
     // From the NSL state invariant
     get_label n_b = join (principal_label alice) (principal_label bob) /\
     // From the PrivateKeys invariant
-    is_decryption_key "NSL.PublicKey" (principal_label bob) tr sk_b /\
+    is_decryption_key (PkdecKey "NSL.PublicKey" empty) (principal_label bob) tr sk_b /\
     // From the network
     bytes_invariant tr msg_cipher
   )
